lib/generic_mm_lemmas.dfy
@@ -1,5 +1,6 @@
 include "generic_bv_ops.dfy"
 include "bv256_ops.dfy"
+include "../arch/otbn/machine.s.dfy"
 
 abstract module generic_mm_lemmas {
     import opened GBV: generic_bv_ops
@@ -7,7 +8,7 @@ abstract module generic_mm_lemmas {
     import opened Mul
     import opened Power
     import opened DivMod
-    import integers
+    import opened integers
 
     type uint = GBV.BVSEQ.uint
 
@@ -28,7 +29,7 @@ abstract module generic_mm_lemmas {
         IsModEquivalent(x, y, BASE())
     }
 
-    function BASE_POW(e: nat): nat
+    function pow_BASE(e: nat): nat
     {
         LemmaPowPositiveAuto();
         Pow(BASE(), e)
@@ -52,7 +53,7 @@ abstract module generic_mm_lemmas {
         && cong_BASE(rsa.M0D * rsa.M, -1)
         // signature
         && 0 < rsa.SIG < rsa.M
-        && rsa.R == BASE_POW(NUM_WORDS)
+        && rsa.R == pow_BASE(NUM_WORDS)
         && rsa.RR < rsa.M
         && IsModEquivalent(rsa.RR, rsa.R * rsa.R, rsa.M)
         && rsa.R_INV == Pow(rsa.BASE_INV, NUM_WORDS)
@@ -91,14 +92,17 @@ abstract module generic_mm_lemmas {
     lemma dw_add_lemma(
         x_lh: uint, x_uh: uint,
         y_lh: uint, y_uh: uint,
-        c1: integers.uint1, c2: integers.uint1,
+        c1: uint1, c2: uint1,
         z_lh: uint, z_uh: uint)
+    returns (z: dw_view_t)
 
         requires dw_add_is_safe(x_lh, x_uh, y_lh, y_uh);
         requires (z_lh, c1) == GBV.addc(x_lh, y_lh, 0);
         requires (z_uh, c2) == GBV.addc(x_uh, y_uh, c1);
         
-        ensures to_nat([z_lh, z_uh]) == to_nat([x_lh, x_uh]) + to_nat([y_lh, y_uh]);
+        ensures z.full == to_nat([z_lh, z_uh]) == to_nat([x_lh, x_uh]) + to_nat([y_lh, y_uh]);
+        ensures z.lh ==  z_lh;
+        ensures z.uh ==  z_uh;
     {
         var x_full := to_nat([x_lh, x_uh]);
         var y_full := to_nat([y_lh, y_uh]);
@@ -110,7 +114,7 @@ abstract module generic_mm_lemmas {
         }
 
         assert GBV.BVSEQ.SeqAdd([x_lh, x_uh], [y_lh, y_uh]) == ([z_lh, z_uh], c2) by {
-            reveal GBV.BVSEQ.SeqAdd();
+            reveal BVSEQ.SeqAdd();
             assert [z_lh] + [z_uh] == [z_lh, z_uh];
         }
 
@@ -122,15 +126,32 @@ abstract module generic_mm_lemmas {
             reveal Pow();
             assert false;
         }
+
+        var full := to_nat([z_lh, z_uh]);
+
+        assert z_lh + z_uh * BASE() == full by {
+            GBV.BVSEQ.LemmaSeqLen2([z_lh, z_uh]);
+        }
+
+        LemmaFundamentalDivModConverse(full, BASE(), z_uh, z_lh);
+
+        assert z_lh == dw_lh(full) by {
+            reveal dw_lh();
+        }
+        assert z_uh == dw_uh(full) by {
+            reveal dw_uh();
+        }
+
+        z := dw_view_cons(z_lh, z_uh, full);
     }
 
-    method dw_add(x_lh: uint, x_uh: uint, y_lh: uint, y_uh: uint)
-        requires dw_add_is_safe(x_lh, x_uh, y_lh, y_uh);
-    {
-        var (z_lh, c1) := GBV.addc(x_lh, y_lh, 0);
-        var (z_uh, c2) := GBV.addc(x_uh, y_uh, c1);
-        dw_add_lemma(x_lh, x_uh, y_lh, y_uh, c1, c2, z_lh, z_uh);
-    }
+    // method dw_add(x_lh: uint, x_uh: uint, y_lh: uint, y_uh: uint)
+    //     requires dw_add_is_safe(x_lh, x_uh, y_lh, y_uh);
+    // {
+    //     var (z_lh, c1) := GBV.addc(x_lh, y_lh, 0);
+    //     var (z_uh, c2) := GBV.addc(x_uh, y_uh, c1);
+    //     dw_add_lemma(x_lh, x_uh, y_lh, y_uh, c1, c2, z_lh, z_uh);
+    // }
 
 /* end section on double word addtion */
 
@@ -197,7 +218,7 @@ abstract module generic_mm_lemmas {
 
     requires |dst| == |src1| == |src2|;
     requires subb_inv(dst, carry, src1, src2, |dst|);
-    ensures to_nat(dst) == to_nat(src1) - to_nat(src2) + carry * BASE_POW(|dst|);
+    ensures to_nat(dst) == to_nat(src1) - to_nat(src2) + carry * pow_BASE(|dst|);
     ensures carry == 0 <==> to_nat(src1) >= to_nat(src2)
     {
         var index := |dst|;
@@ -207,7 +228,7 @@ abstract module generic_mm_lemmas {
     
         GBV.BVSEQ.LemmaSeqSub(src1, src2, dst, carry);
 
-        assert to_nat(src1) - to_nat(src2) + carry * BASE_POW(index) == to_nat(dst);
+        assert to_nat(src1) - to_nat(src2) + carry * pow_BASE(index) == to_nat(dst);
 
         GBV.BVSEQ.LemmaSeqNatBound(dst);
     }
@@ -306,90 +327,89 @@ abstract module generic_mm_lemmas {
         LemmaSmallMod(p2.lh, BASE());
     }
 
-/*
     predicate mont_loop_inv(
-        xi: uint256,
-        ui: uint256,
+        xi: uint,
+        ui: uint,
         p1: dw_view_t,
         p2: dw_view_t,
-        y: seq<uint256>,
-        m: seq<uint256>,
-        prev_a: seq<uint256>,
-        next_a: seq<uint256>,
+        y: seq<uint>,
+        m: seq<uint>,
+        prev_a: seq<uint>,
+        next_a: seq<uint>,
         j: nat)
     {
         && |m| == |next_a| == |y| == |prev_a| == NUM_WORDS
         && (1 <= j <= NUM_WORDS)
-        && (xi * ToNat(y[..j]) + ui * ToNat(m[..j]) + ToNat(prev_a[..j]) 
+        && (xi * to_nat(y[..j]) + ui * to_nat(m[..j]) + to_nat(prev_a[..j]) 
             == 
-        ToNat([0] + next_a[..j-1]) + p2.uh * pow_B256(j) + p1.uh * pow_B256(j))
+        to_nat([0] + next_a[..j-1]) + p2.uh * pow_BASE(j) + p1.uh * pow_BASE(j))
     }
 
     lemma mont_loop_inv_pre_lemma(
-        xi: uint256,
-        ui: uint256,
-        m0d: uint256,
+        xi: uint,
+        ui: uint,
+        m0d: uint,
         p1: dw_view_t,
         p2: dw_view_t,
-        y: seq<uint256>,
-        m: seq<uint256>,
-        a: seq<uint256>)
+        y: seq<uint>,
+        m: seq<uint>,
+        a: seq<uint>)
+        requires NUM_WORDS > 0;
         requires |m| == |a| == |y| == NUM_WORDS;
         requires p1.full == xi * y[0] + a[0];
         requires p2.full == ui * m[0] + p1.lh;
-        requires cong_BASE(m0d * ToNat(m), -1);
+        requires cong_BASE(m0d * to_nat(m), -1);
         requires cong_BASE(ui, (a[0] + y[0] * xi) * m0d);
 
         ensures mont_loop_inv(xi, ui, p1, p2, y, m, a, a, 1)
     {
         assert cong_BASE(m0d * m[0], -1) by {
-            LemmaSeqLswModEquivalence(m);
-            LemmaModMulEquivalent(ToNat(m), m[0], m0d, BASE());
+            GBV.BVSEQ.LemmaSeqLswModEquivalence(m);
+            LemmaModMulEquivalent(to_nat(m), m[0], m0d, BASE());
             LemmaMulIsCommutativeAuto();
         }
 
         mont_loop_divisible_lemma(ui, m0d, p1, p2, m[0]);
 
-        LemmaSeqLen1(y[..1]);
-        LemmaSeqLen1(m[..1]);
-        LemmaSeqLen1(a[..1]);
+        GBV.BVSEQ.LemmaSeqLen1(y[..1]);
+        GBV.BVSEQ.LemmaSeqLen1(m[..1]);
+        GBV.BVSEQ.LemmaSeqLen1(a[..1]);
 
         assert p2.full == p2.uh * BASE() by {
-            uint512_view_lemma(p2);
+            dw_view_lemma(p2);
         }
 
-        uint512_view_lemma(p1);
+        dw_view_lemma(p1);
 
         calc {
-            xi * ToNat(y[..1]) + ui * ToNat(m[..1]) + ToNat(a[..1]);
+            xi * to_nat(y[..1]) + ui * to_nat(m[..1]) + to_nat(a[..1]);
                 { reveal Pow(); }
-            p2.uh * pow_B256(1) + p1.uh * pow_B256(1);
+            p2.uh * pow_BASE(1) + p1.uh * pow_BASE(1);
                 {
-                    reveal ToNatRight();
-                    assert ToNat([0]) == 0;
+                    reveal GBV.BVSEQ.ToNatRight();
+                    assert to_nat([0]) == 0;
                 }
-            ToNat([0]) + p2.uh * pow_B256(1) + p1.uh * pow_B256(1);
+            to_nat([0]) + p2.uh * pow_BASE(1) + p1.uh * pow_BASE(1);
                 {
                     assert [0] + a[..0] == [0];
-                    assert ToNat([0]) == ToNat([0] + a[..0]);
+                    assert to_nat([0]) == to_nat([0] + a[..0]);
                 }
-            ToNat([0] + a[..0]) + p2.uh * pow_B256(1) + p1.uh * pow_B256(1);
-
+            to_nat([0] + a[..0]) + p2.uh * pow_BASE(1) + p1.uh * pow_BASE(1);
         }
     }
 
     lemma mont_loop_inv_peri_lemma(
-        xi: uint256,
-        ui: uint256,
+        xi: uint,
+        ui: uint,
         p1: dw_view_t,
         p2: dw_view_t,
         next_p1: dw_view_t,
         next_p2: dw_view_t,
-        y: seq<uint256>,
-        m: seq<uint256>,
-        prev_a: seq<uint256>,
-        a: seq<uint256>,
-        next_a: seq<uint256>,
+        y: seq<uint>,
+        m: seq<uint>,
+        prev_a: seq<uint>,
+        a: seq<uint>,
+        next_a: seq<uint>,
         j: nat)
 
         requires 1 <= j < NUM_WORDS; // this is in the loop itself
@@ -401,82 +421,89 @@ abstract module generic_mm_lemmas {
         requires next_a == a[j-1 := next_p2.lh];
         ensures mont_loop_inv(xi, ui, next_p1, next_p2, y, m, prev_a, next_a, j+1);
     {
-        var y_nat := ToNat(y[..j]);
-        var y_nat' := ToNat(y[..j+1]);
+        var y_nat := to_nat(y[..j]);
+        var y_nat' := to_nat(y[..j+1]);
         var y_j := y[j];
 
-        var m_nat := ToNat(m[..j]);
-        var m_nat' := ToNat(m[..j+1]);
+        var m_nat := to_nat(m[..j]);
+        var m_nat' := to_nat(m[..j+1]);
         var m_j := m[j];
 
-        var ia_nat := ToNat(prev_a[..j]);
-        var ia_nat' := ToNat(prev_a[..j+1]);
+        var ia_nat := to_nat(prev_a[..j]);
+        var ia_nat' := to_nat(prev_a[..j+1]);
         var a_j := prev_a[j];
 
-        var ea_nat := ToNat([0] + a[..j-1]);
-        var ea_nat' := ToNat([0] + next_a[..j]);
+        var ea_nat := to_nat([0] + a[..j-1]);
+        var ea_nat' := to_nat([0] + next_a[..j]);
 
-        var pow_B256_j := pow_B256(j);
-        var pow_B256_j' := pow_B256(j+1);
+        var pow_BASE_j := pow_BASE(j);
+        var pow_BASE_j' := pow_BASE(j+1);
 
         var p1_uh := p1.uh;
         var p2_uh := p2.uh;
 
-        assert pow_B256_j' == pow_B256_j * BASE() by {
-          reveal Pow();
+        assert pow_BASE_j' == pow_BASE_j * BASE() by {
+            LemmaMulIsCommutative(pow_BASE_j, BASE());
+            reveal Pow();
         }
 
         assert xi * y_nat + ui * m_nat + ia_nat 
             == 
-        ea_nat + p2_uh * pow_B256_j +p1_uh * pow_B256_j;
+        ea_nat + p2_uh * pow_BASE_j +p1_uh * pow_BASE_j;
 
         assert p1_uh == next_p1.lh + next_p1.uh * BASE() - y_j * xi - a_j by {
-            uint512_view_lemma(next_p1);
+            dw_view_lemma(next_p1);
         }
 
         assert p2_uh == next_p2.lh + next_p2.uh * BASE() - m_j * ui - next_p1.lh by {
-            uint512_view_lemma(next_p2);
+            dw_view_lemma(next_p2);
         }
 
-        assert ia_nat' == ia_nat + a_j * pow_B256_j by {
+        assert ia_nat' == ia_nat + a_j * pow_BASE_j by {
             assert prev_a[..j+1][..j] == prev_a[..j];
-            LemmaToNatLeftEqToNatRightAuto();
-            reveal ToNatLeft();
+            GBV.BVSEQ.LemmaToNatLeftEqToNatRightAuto();
+            reveal GBV.BVSEQ.ToNatLeft();
         }
 
-        assert y_nat' == y_nat + y_j * pow_B256_j by {
+        assert y_nat' == y_nat + y_j * pow_BASE_j by {
             assert y[..j+1][..j] == y[..j];
-            LemmaToNatLeftEqToNatRightAuto();
-            reveal ToNatLeft();
+            GBV.BVSEQ.LemmaToNatLeftEqToNatRightAuto();
+            reveal GBV.BVSEQ.ToNatLeft();
         }
 
-        assert m_nat' == m_nat + m_j * pow_B256_j by {
+        assert m_nat' == m_nat + m_j * pow_BASE_j by {
             assert m[..j+1][..j] == m[..j];
-            LemmaToNatLeftEqToNatRightAuto();
-            reveal ToNatLeft();
+            GBV.BVSEQ.LemmaToNatLeftEqToNatRightAuto();
+            reveal GBV.BVSEQ.ToNatLeft();
         }
 
-        assert ea_nat' == ea_nat + next_p2.lh * pow_B256_j by {
+        assert ea_nat' == ea_nat + next_p2.lh * pow_BASE_j by {
             calc == {
-                ToNat(next_a[..j]);
+                to_nat(next_a[..j]);
                     {
-                        LemmaSeqPrefix(next_a[..j], j - 1);
+                        GBV.BVSEQ.LemmaSeqPrefix(next_a[..j], j - 1);
                         assert next_a[..j-1] == next_a[..j][..j-1];
-                        reveal ToNatRight();
+                        reveal GBV.BVSEQ.ToNatRight();
                     }
-                ToNat(next_a[..j-1]) + next_p2.lh * pow_B256(j-1);
-                ToNat(a[..j-1]) + next_p2.lh * pow_B256(j-1);
+                to_nat(next_a[..j-1]) + next_p2.lh * pow_BASE(j-1);
+                to_nat(a[..j-1]) + next_p2.lh * pow_BASE(j-1);
             }
 
-            assert ToNat([0] + a[..j-1]) == ToNat(a[..j-1]) * BASE() by {
-                reveal ToNatRight();
+            assert ea_nat == to_nat([0] + a[..j-1]) == to_nat(a[..j-1]) * BASE() by {
+                reveal GBV.BVSEQ.ToNatRight();
+            }
+            
+            calc == {
+                ea_nat';
+                to_nat([0] + next_a[..j]);
+                    { reveal GBV.BVSEQ.ToNatRight(); }
+                to_nat(next_a[..j]) * BASE();
+                (to_nat(a[..j-1]) + next_p2.lh * pow_BASE(j-1)) * BASE();
+                    { LemmaMulIsDistributiveAddOtherWayAuto(); }
+                to_nat(a[..j-1]) * BASE() + next_p2.lh * pow_BASE(j-1) * BASE();
             }
 
-            assert ToNat([0] + next_a[..j]) == ToNat(next_a[..j]) * BASE() by {
-                reveal ToNatRight();
-            }
-
-            assert pow_B256(j-1) * BASE() == pow_B256(j) by {
+            assert pow_BASE(j-1) * BASE() == pow_BASE(j) by {
                 reveal Pow();
             }
 
@@ -485,148 +512,176 @@ abstract module generic_mm_lemmas {
 
         assert xi * y_nat' + ui * m_nat' + ia_nat'
             ==
-        ea_nat' + next_p2.uh * pow_B256_j' + next_p1.uh * pow_B256_j' by {
+        ea_nat' + next_p2.uh * pow_BASE_j' + next_p1.uh * pow_BASE_j' by {
             LemmaMulProperties();
         }
     }
 
     lemma mont_loop_inv_post_lemma(
-        xi: uint256,
-        ui: uint256,
+        xi: uint,
+        ui: uint,
         p1: dw_view_t,
         p2: dw_view_t,
-        y: seq<uint256>,
-        m: seq<uint256>,
-        prev_a: seq<uint256>,
-        a: seq<uint256>,
+        y: seq<uint>,
+        m: seq<uint>,
+        prev_a: seq<uint>,
+        a: seq<uint>,
         bout: uint1)
 
+        requires NUM_WORDS > 0;
         requires mont_loop_inv(xi, ui, p1, p2, y, m, prev_a, a, NUM_WORDS);
-        requires uint256_addc(p1.uh, p2.uh, 0) == (a[NUM_WORDS-1], bout);
+        requires GBV.addc(p1.uh, p2.uh, 0) == (a[NUM_WORDS-1], bout);
 
-        ensures ToNat(a) * BASE() + bout * pow_B256(NUM_WORDS+1)
-            == xi * ToNat(y) + ui * ToNat(m) + ToNat(prev_a);
+        ensures to_nat(a) * BASE() + bout * pow_BASE(NUM_WORDS+1)
+            == xi * to_nat(y) + ui * to_nat(m) + to_nat(prev_a);
     {
-        // var m := ToNat(m);
+        // var m := to_nat(m);
         calc {
-            ToNat(a) * BASE() + bout * pow_B256(NUM_WORDS+1);
+            to_nat(a) * BASE() + bout * pow_BASE(NUM_WORDS+1);
                 {
-                    LemmaToNatLeftEqToNatRight(a);
-                    reveal ToNatLeft();
-                    LemmaToNatLeftEqToNatRight(a[..NUM_WORDS-1]);
+                    GBV.BVSEQ.LemmaToNatLeftEqToNatRight(a);
+                    reveal GBV.BVSEQ.ToNatLeft();
+                    GBV.BVSEQ.LemmaToNatLeftEqToNatRight(a[..NUM_WORDS-1]);
                 }
-            (ToNat(a[..NUM_WORDS-1]) + a[NUM_WORDS-1] * pow_B256(NUM_WORDS-1)) * BASE() + bout * pow_B256(NUM_WORDS+1);
-            ToNat(a[..NUM_WORDS-1]) * BASE() + a[NUM_WORDS-1] * pow_B256(NUM_WORDS-1) * BASE() + bout * pow_B256(NUM_WORDS+1);
+            (to_nat(a[..NUM_WORDS-1]) + a[NUM_WORDS-1] * pow_BASE(NUM_WORDS-1)) * BASE() + bout * pow_BASE(NUM_WORDS+1);
+                { LemmaMulIsDistributiveAddOtherWayAuto(); }
+            to_nat(a[..NUM_WORDS-1]) * BASE() + a[NUM_WORDS-1] * pow_BASE(NUM_WORDS-1) * BASE() + bout * pow_BASE(NUM_WORDS+1);
                 {
                     reveal Pow();
                     LemmaMulIsCommutativeAuto();
                     LemmaMulIsAssociativeAuto();
                 }
-            ToNat(a[..NUM_WORDS-1]) * BASE() + a[NUM_WORDS-1] * pow_B256(NUM_WORDS) + bout * BASE() * pow_B256(NUM_WORDS);
+            to_nat(a[..NUM_WORDS-1]) * BASE() + a[NUM_WORDS-1] * pow_BASE(NUM_WORDS) + bout * BASE() * pow_BASE(NUM_WORDS);
                 { LemmaMulIsDistributiveAuto(); }
-            ToNat(a[..NUM_WORDS-1]) * BASE() + p2.uh * pow_B256(NUM_WORDS) + p1.uh * pow_B256(NUM_WORDS);
-                { reveal ToNatRight(); }
-            ToNat([0] + a[..NUM_WORDS-1]) + p2.uh * pow_B256(NUM_WORDS) + p1.uh * pow_B256(NUM_WORDS);
+            to_nat(a[..NUM_WORDS-1]) * BASE() + p2.uh * pow_BASE(NUM_WORDS) + p1.uh * pow_BASE(NUM_WORDS);
+                { reveal GBV.BVSEQ.ToNatRight(); }
+            to_nat([0] + a[..NUM_WORDS-1]) + p2.uh * pow_BASE(NUM_WORDS) + p1.uh * pow_BASE(NUM_WORDS);
                 {
                     assert y == y[..NUM_WORDS];
                     assert m == m[..NUM_WORDS];
                     assert prev_a == prev_a[..NUM_WORDS];
                 }
-            xi * ToNat(y) + ui * ToNat(m) + ToNat(prev_a);
+            xi * to_nat(y) + ui * to_nat(m) + to_nat(prev_a);
         }
     }
 
-    lemma mont_loop_cond_sub_borrow_lemma(xi: uint256,
-        ui: uint256,
-        y: seq<uint256>,
+    lemma mont_loop_cond_sub_borrow_lemma(xi: uint,
+        ui: uint,
+        y: seq<uint>,
         m: nat,
         prev_a: nat,
-        a: seq<uint256>,
-        next_a: seq<uint256>,
+        a: seq<uint>,
+        next_a: seq<uint>,
         next_bout: uint1)
 
         requires m != 0;
         requires |next_a| == |y| == NUM_WORDS;
-        requires prev_a < m + ToNat(y);
-        requires ToNat(a) * BASE() + pow_B256(NUM_WORDS+1)
-            == xi * ToNat(y) + ui * m + prev_a;
-        requires ToNat(next_a) - pow_B256(NUM_WORDS) * next_bout == ToNat(a) - m
-        requires ToNat(a) + pow_B256(NUM_WORDS) < ToNat(y) + m
+        requires prev_a < m + to_nat(y);
+        requires to_nat(a) * BASE() + pow_BASE(NUM_WORDS+1)
+            == xi * to_nat(y) + ui * m + prev_a;
+        requires to_nat(next_a) - pow_BASE(NUM_WORDS) * next_bout == to_nat(a) - m
+        requires to_nat(a) + pow_BASE(NUM_WORDS) < to_nat(y) + m
 
-        ensures ToNat(next_a) < m + ToNat(y)
-        ensures IsModEquivalent(ToNat(next_a) * BASE(), xi * ToNat(y) + ui * m + prev_a, m)
+        ensures to_nat(next_a) < m + to_nat(y)
+        ensures IsModEquivalent(to_nat(next_a) * BASE(), xi * to_nat(y) + ui * m + prev_a, m)
     {
-        if ToNat(a) >= m {
-            LemmaSeqNatBound(y);
-            assert ToNat(a) + pow_B256(NUM_WORDS) < ToNat(y) + m;
+        if to_nat(a) >= m {
+            GBV.BVSEQ.LemmaSeqNatBound(y);
+            assert to_nat(a) + pow_BASE(NUM_WORDS) < to_nat(y) + m;
             assert false; // prove by contradiction
         }
         if next_bout != 1 {
-            LemmaSeqNatBound(next_a);
+            GBV.BVSEQ.LemmaSeqNatBound(next_a);
             assert false; // prove by contradiction
         }
         
         assert next_bout == 1;
 
         calc {
-            ToNat(next_a) * BASE();
-            ToNat(a) * BASE() + pow_B256(NUM_WORDS) * BASE() - m * BASE();
-                { reveal Pow(); }
-            ToNat(a) * BASE() + pow_B256(NUM_WORDS+1) - m * BASE();
-            xi * ToNat(y) + ui * m + prev_a - m * BASE();
+            to_nat(next_a) * BASE();
+            (to_nat(a) + pow_BASE(NUM_WORDS) * next_bout - m) * BASE();
+            (to_nat(a) - m + pow_BASE(NUM_WORDS) * next_bout) * BASE();
+                { LemmaMulIsDistributive(BASE(), to_nat(a) - m, pow_BASE(NUM_WORDS) * next_bout); }
+            (to_nat(a) - m) * BASE() + (pow_BASE(NUM_WORDS) * next_bout) * BASE();
+            (to_nat(a) - m) * BASE() + pow_BASE(NUM_WORDS) * BASE() * next_bout;
+                {
+                    reveal Pow();
+                    LemmaMulIsCommutativeAuto();
+                    assert pow_BASE(NUM_WORDS) * BASE() == pow_BASE(NUM_WORDS + 1);
+                }
+            (to_nat(a) - m) * BASE() + pow_BASE(NUM_WORDS+1) * next_bout;
+                { LemmaMulIsDistributive(BASE(), to_nat(a), m); }
+            to_nat(a) * BASE() - m * BASE() + pow_BASE(NUM_WORDS+1) * next_bout;
+            xi * to_nat(y) + ui * m + prev_a - m * BASE();
         }
         
         calc ==> {
             true;
-            IsModEquivalent(ToNat(next_a) * BASE(), xi * ToNat(y) + ui * m + prev_a - m * BASE(), m);
-                { LemmaModMultiplesVanish(-1 * BASE(), xi * ToNat(y) + ui * m + prev_a, m); }
-            IsModEquivalent(ToNat(next_a) * BASE(), xi * ToNat(y) + ui * m + prev_a, m);
+            IsModEquivalent(to_nat(next_a) * BASE(), xi * to_nat(y) + ui * m + prev_a - m * BASE(), m);
+                {
+                    LemmaModMultiplesVanish(-1 * BASE(), xi * to_nat(y) + ui * m + prev_a, m);
+                    LemmaMulIsAssociativeAuto();
+                    LemmaMulIsCommutativeAuto();
+                }
+            IsModEquivalent(to_nat(next_a) * BASE(), xi * to_nat(y) + ui * m + prev_a, m);
         }
     }
 
     lemma mont_loop_cond_sub_lemma(
-        xi: uint256,
-        ui: uint256,
-        y: seq<uint256>,
+        xi: uint,
+        ui: uint,
+        y: seq<uint>,
         m: nat,
         prev_a: nat,
-        a: seq<uint256>,
-        next_a: seq<uint256>,
+        a: seq<uint>,
+        next_a: seq<uint>,
         bout: uint1,
         next_bout: uint1)
 
         requires m != 0;
         requires |next_a| == |y| == NUM_WORDS;
-        requires prev_a < m + ToNat(y);
-        requires ToNat(a) * BASE() + bout * pow_B256(NUM_WORDS+1)
-            == xi * ToNat(y) + ui * m + prev_a;
+        requires prev_a < m + to_nat(y);
+        requires to_nat(a) * BASE() + bout * pow_BASE(NUM_WORDS+1)
+            == xi * to_nat(y) + ui * m + prev_a;
         requires bout == 0 ==>
-            ToNat(a) == ToNat(next_a)
+            to_nat(a) == to_nat(next_a)
         requires bout == 1 ==>
-            ToNat(next_a) - pow_B256(NUM_WORDS) * next_bout == ToNat(a) - m
+            to_nat(next_a) - pow_BASE(NUM_WORDS) * next_bout == to_nat(a) - m
 
-        ensures ToNat(next_a) < m + ToNat(y)
-        ensures IsModEquivalent(ToNat(next_a) * BASE(), xi * ToNat(y) + ui * m + prev_a, m)
+        ensures to_nat(next_a) < m + to_nat(y)
+        ensures IsModEquivalent(to_nat(next_a) * BASE(), xi * to_nat(y) + ui * m + prev_a, m)
     {
-        assert ToNat(a) + bout * pow_B256(NUM_WORDS) < ToNat(y) + m by {
+        if to_nat(a) + bout * pow_BASE(NUM_WORDS) >= to_nat(y) + m {
             calc {
-                (ToNat(a) + bout * pow_B256(NUM_WORDS)) * BASE();
-                ToNat(a) * BASE() + bout * pow_B256(NUM_WORDS) * BASE();
-                    { reveal Pow(); }
-                ToNat(a) * BASE() + bout * pow_B256(NUM_WORDS+1);
-                xi * ToNat(y) + ui * m + prev_a;
-                <
-                xi * ToNat(y) + ui * m + m + ToNat(y);
+                (to_nat(a) + bout * pow_BASE(NUM_WORDS)) * BASE();
                     { LemmaMulIsDistributiveAuto(); }
-                (xi + 1) * ToNat(y) + (ui + 1) * m;
+                to_nat(a) * BASE() + bout * pow_BASE(NUM_WORDS) * BASE();
+                    {
+                        reveal Pow();
+                        LemmaMulIsAssociativeAuto();
+                    }
+                to_nat(a) * BASE() + bout * pow_BASE(NUM_WORDS+1);
+                xi * to_nat(y) + ui * m + prev_a;
+                <
+                xi * to_nat(y) + ui * m + m + to_nat(y);
+                    { LemmaMulIsDistributiveAuto(); }
+                (xi + 1) * to_nat(y) + (ui + 1) * m;
                 <=  {
                         assert xi + 1 <= BASE();
                         assert ui + 1 <= BASE();
                         LemmaMulInequalityConverseAuto();
                     }
-                BASE() * ToNat(y) + BASE() * m;
-                (ToNat(y) + m) * BASE();
+                BASE() * to_nat(y) + BASE() * m;
+                    { LemmaMulIsDistributiveAuto(); }
+                (to_nat(y) + m) * BASE();
             }
+
+            if to_nat(y) + m < to_nat(a) + bout * pow_BASE(NUM_WORDS) {
+                LemmaMulStrictInequality(to_nat(y) + m, to_nat(a) + bout * pow_BASE(NUM_WORDS), BASE());
+                assert false;
+            }
+
+            assert false;
         }
         
         if bout == 1 {
@@ -634,81 +689,459 @@ abstract module generic_mm_lemmas {
         }
     }
 
+/* end section on mont loop */
+
+/* begin section on mont mul */
+
     predicate montmul_inv(
-        a: seq<uint256>,
-        x: seq<uint256>,
+        a: seq<uint>,
+        x: seq<uint>,
         i: nat,
-        y: seq<uint256>,
+        y: seq<uint>,
         rsa: rsa_params)
     {
         && |a| == |y| == |x| == NUM_WORDS
         && i <= |x|
         && rsa_params_inv(rsa)
-        && ToNat(a) < rsa.M + ToNat(y)
-        && IsModEquivalent(ToNat(a) * pow_B256(i), ToNat(x[..i]) * ToNat(y), rsa.M)
+        && to_nat(a) < rsa.M + to_nat(y)
+        && IsModEquivalent(to_nat(a) * pow_BASE(i), to_nat(x[..i]) * to_nat(y), rsa.M)
     }
 
     lemma montmul_inv_lemma(
-        prev_a: seq<uint256>,
-        a: seq<uint256>,
-        x: seq<uint256>, 
+        prev_a: seq<uint>,
+        a: seq<uint>,
+        x: seq<uint>, 
         i: nat,
         ui: int,
-        y: seq<uint256>, 
+        y: seq<uint>, 
         rsa: rsa_params)
 
         requires montmul_inv(prev_a, x, i, y, rsa);
         requires |a| == NUM_WORDS;
         requires i < |x|;
-        requires ToNat(a) < rsa.M + ToNat(y);
-        requires IsModEquivalent(ToNat(a) * pow_B256(1),
-                x[i] * ToNat(y) + ui * rsa.M + ToNat(prev_a), rsa.M);
+        requires to_nat(a) < rsa.M + to_nat(y);
+        requires IsModEquivalent(to_nat(a) * pow_BASE(1),
+                x[i] * to_nat(y) + ui * rsa.M + to_nat(prev_a), rsa.M);
         ensures montmul_inv(a, x, i+1, y, rsa);
     {
-        var curr_a := ToNat(a);
-        var prev_a := ToNat(prev_a);
+        var curr_a := to_nat(a);
+        var prev_a := to_nat(prev_a);
         calc ==> {
-            IsModEquivalent(curr_a * pow_B256(1), x[i] * ToNat(y) + ui * rsa.M + prev_a, rsa.M);
+            IsModEquivalent(curr_a * pow_BASE(1), x[i] * to_nat(y) + ui * rsa.M + prev_a, rsa.M);
                 {
                     LemmaMulIsCommutativeAuto();
-                    LemmaModMultiplesVanish(ui, x[i] * ToNat(y) + prev_a, rsa.M);
+                    LemmaModMultiplesVanish(ui, x[i] * to_nat(y) + prev_a, rsa.M);
                 }
-            IsModEquivalent(curr_a * pow_B256(1), x[i] * ToNat(y) + prev_a, rsa.M);
+            IsModEquivalent(curr_a * pow_BASE(1), x[i] * to_nat(y) + prev_a, rsa.M);
                 {
-                    LemmaModMulEquivalent(curr_a * pow_B256(1), x[i] * ToNat(y) + prev_a, pow_B256(i), rsa.M);
+                    LemmaModMulEquivalent(curr_a * pow_BASE(1), x[i] * to_nat(y) + prev_a, pow_BASE(i), rsa.M);
                     LemmaMulIsDistributiveAuto();
                 }
-            IsModEquivalent(curr_a * pow_B256(1) * pow_B256(i), x[i] * ToNat(y) * pow_B256(i) + prev_a * pow_B256(i), rsa.M);
+            IsModEquivalent(curr_a * pow_BASE(1) * pow_BASE(i), x[i] * to_nat(y) * pow_BASE(i) + prev_a * pow_BASE(i), rsa.M);
                 {
                     reveal Pow();
                     LemmaMulIsAssociativeAuto();
                 }
-            IsModEquivalent(curr_a * pow_B256(1+i), x[i] * ToNat(y) * pow_B256(i) + prev_a * pow_B256(i), rsa.M);
+            IsModEquivalent(curr_a * pow_BASE(1+i), x[i] * to_nat(y) * pow_BASE(i) + prev_a * pow_BASE(i), rsa.M);
                 {
-                    LemmaAddModNoopRight(x[i] * ToNat(y) * pow_B256(i), prev_a * pow_B256(i), rsa.M);
-                    LemmaAddModNoopRight(x[i] * ToNat(y) * pow_B256(i), ToNat(x[..i]) * ToNat(y), rsa.M);
+                    LemmaAddModNoopRight(x[i] * to_nat(y) * pow_BASE(i), prev_a * pow_BASE(i), rsa.M);
+                    LemmaAddModNoopRight(x[i] * to_nat(y) * pow_BASE(i), to_nat(x[..i]) * to_nat(y), rsa.M);
                 }
-            IsModEquivalent(curr_a * pow_B256(1+i), x[i] * ToNat(y) * pow_B256(i) + ToNat(x[..i]) * ToNat(y), rsa.M);
+            IsModEquivalent(curr_a * pow_BASE(1+i), x[i] * to_nat(y) * pow_BASE(i) + to_nat(x[..i]) * to_nat(y), rsa.M);
                 { LemmaMulProperties(); }
-            IsModEquivalent(curr_a * pow_B256(1+i), (x[i] * pow_B256(i) + ToNat(x[..i])) * ToNat(y), rsa.M);
+            IsModEquivalent(curr_a * pow_BASE(1+i), (x[i] * pow_BASE(i) + to_nat(x[..i])) * to_nat(y), rsa.M);
                 {
                     assert x[..i+1][..i] == x[..i];
-                    LemmaToNatLeftEqToNatRightAuto();
-                    reveal ToNatLeft();
+                    GBV.BVSEQ.LemmaToNatLeftEqToNatRightAuto();
+                    reveal GBV.BVSEQ.ToNatLeft();
                 }
-            IsModEquivalent(curr_a * pow_B256(1+i), ToNat(x[..i+1]) * ToNat(y), rsa.M);
+            IsModEquivalent(curr_a * pow_BASE(1+i), to_nat(x[..i+1]) * to_nat(y), rsa.M);
         }
 
-        assert IsModEquivalent(curr_a * pow_B256(1+i), ToNat(x[..i+1]) * ToNat(y), rsa.M);
+        assert IsModEquivalent(curr_a * pow_BASE(1+i), to_nat(x[..i+1]) * to_nat(y), rsa.M);
     }
-    */
 
-/* end section on mont loop */
+    lemma montmul_inv_lemma_0(
+        a: seq<uint>,
+        x: seq<uint>, 
+        i: nat,
+        y: seq<uint>, 
+        rsa: rsa_params)
+
+        requires |a| == |x| == |y| == NUM_WORDS;
+        requires to_nat(a) == 0;
+        requires rsa_params_inv(rsa);
+        requires i == 0;
+        
+        ensures montmul_inv(a, x, i, y, rsa);
+    {
+        assert to_nat(x[..i]) == 0 by {
+            reveal GBV.BVSEQ.ToNatRight();
+        }
+        assert montmul_inv(a, x, i, y, rsa);
+    }
+
+    lemma r_r_inv_cancel_lemma(a: nat, b: nat, rsa: rsa_params)
+        requires rsa_params_inv(rsa);
+        requires IsModEquivalent(a, b * rsa.R_INV * rsa.R, rsa.M);
+        ensures IsModEquivalent(a, b, rsa.M);
+    {
+        assert IsModEquivalent(b * rsa.R_INV * rsa.R, b, rsa.M) by {
+            LemmaModMulEquivalent(rsa.R_INV * rsa.R, 1, b, rsa.M);
+            LemmaMulIsAssociativeAuto();
+        }
+    }
+
+    lemma montmul_inv_lemma_1(
+        a_view: seq<uint>,
+        x: seq<uint>,
+        y: seq<uint>,
+        rsa: rsa_params)
+    
+        requires montmul_inv(a_view, x, NUM_WORDS, y, rsa);
+        ensures IsModEquivalent(to_nat(a_view), to_nat(x) * to_nat(y) * rsa.R_INV, rsa.M);
+    {
+        var m := rsa.M;
+        var a := to_nat(a_view);
+        assert x[..NUM_WORDS] == x;
+
+        calc ==> {
+            IsModEquivalent(a * rsa.R, to_nat(x) * to_nat(y), m);
+                { LemmaModMulEquivalentAuto(); }
+            IsModEquivalent(a * rsa.R * rsa.R_INV, to_nat(x) * to_nat(y) * rsa.R_INV, m);
+            IsModEquivalent(to_nat(x) * to_nat(y) * rsa.R_INV, a * rsa.R * rsa.R_INV, m);
+                {
+                    LemmaMulIsAssociativeAuto();
+                    LemmaMulNonnegativeAuto();
+                    r_r_inv_cancel_lemma(to_nat(x) * to_nat(y) * rsa.R_INV, a, rsa);
+                }
+            IsModEquivalent(to_nat(x) * to_nat(y) * rsa.R_INV, a, m);
+            IsModEquivalent(a, to_nat(x) * to_nat(y) * rsa.R_INV, m);
+        }
+    }
+
+/* end section on mont mul */
+
+/* start section on mont mod exp */
+
+    predicate modexp_var_inv(
+        a: nat,
+        sig: nat,
+        i: nat,
+        rsa: rsa_params)
+        requires rsa.M != 0;
+    {
+        LemmaPowPositiveAuto();
+        IsModEquivalent(a, Pow(sig, Pow(2, i)) * rsa.R, rsa.M)
+    }
+
+    lemma modexp_var_inv_pre_lemma(
+        a_view: seq<uint>,
+        rr: seq<uint>,
+        sig: seq<uint>,
+        rsa: rsa_params)
+
+    requires montmul_inv(a_view, rr, NUM_WORDS, sig, rsa);
+    requires to_nat(rr) == rsa.RR;
+    ensures modexp_var_inv(to_nat(a_view), to_nat(sig), 0, rsa);
+    {
+        var m := rsa.M;
+        var a := to_nat(a_view);
+        var s := to_nat(sig);
+
+        calc ==> {
+            true;
+                { LemmaModMulEquivalentAuto(); }
+            IsModEquivalent(rsa.RR * rsa.R_INV, rsa.R * rsa.R * rsa.R_INV, m);
+                {
+                    LemmaMulProperties();
+                    r_r_inv_cancel_lemma(rsa.RR * rsa.R_INV, rsa.R, rsa);
+                }
+            IsModEquivalent(rsa.RR * rsa.R_INV, rsa.R, m);
+        }
+
+        assert IsModEquivalent(a, s * rsa.R, m) by {
+            assert IsModEquivalent(rsa.RR * rsa.R_INV * s, rsa.R * s, m) by {
+                LemmaModMulEquivalentAuto();
+            }
+            assert IsModEquivalent(a, rsa.RR * rsa.R_INV * s, m) by {
+                montmul_inv_lemma_1(a_view, rr, sig, rsa);
+                LemmaMulProperties();
+            }
+        }
+        
+        reveal Pow();
+    }
+
+    lemma modexp_var_inv_peri_lemma(
+        a_view: seq<uint>,
+        next_a_view: seq<uint>,
+        sig: nat,
+        i: nat,
+        rsa: rsa_params)
+
+        requires montmul_inv(next_a_view, a_view, NUM_WORDS, a_view, rsa);
+        requires sig > 0;
+        requires modexp_var_inv(to_nat(a_view), sig, i, rsa);
+        ensures modexp_var_inv(to_nat(next_a_view), sig, i + 1, rsa);
+    {
+        var m := rsa.M;
+        var a := to_nat(a_view);
+        var next_a := to_nat(next_a_view);
+
+        LemmaPowPositiveAuto();
+        // LemmaPowNonnegativeAuto();
+        LemmaMulNonnegativeAuto();
+        var next_goal := Pow(sig, Pow(2, i + 1)) * rsa.R;
+
+        assert IsModEquivalent(a, Pow(sig, Pow(2, i)) * rsa.R, m);
+        
+        calc ==> {
+            IsModEquivalent(a, Pow(sig, Pow(2, i)) * rsa.R, m);
+                {
+                    LemmaMulModNoop(a, a, m);
+                    LemmaMulModNoop(Pow(sig, Pow(2, i)) * rsa.R, Pow(sig, Pow(2, i)) * rsa.R, m);
+                    LemmaMulProperties();
+                }
+            IsModEquivalent(a * a, Pow(sig, Pow(2, i)) * rsa.R * Pow(sig, Pow(2, i)) * rsa.R, m);
+                { LemmaMulIsAssociativeAuto(); }
+            IsModEquivalent(a * a, Pow(sig, Pow(2, i)) * Pow(sig, Pow(2, i)) * rsa.R * rsa.R, m);
+                { LemmaPowAddsAuto(); }
+            IsModEquivalent(a * a, Pow(sig, Pow(2, i) + Pow(2, i)) * rsa.R * rsa.R, m);
+                { reveal Pow(); }
+            IsModEquivalent(a * a, next_goal * rsa.R, m);
+                { LemmaModMulEquivalentAuto(); }
+            IsModEquivalent(a * a * rsa.R_INV, next_goal * rsa.R * rsa.R_INV, m);
+                {
+                    assert IsModEquivalent(next_a, a * a * rsa.R_INV, m) by {
+                        montmul_inv_lemma_1(next_a_view, a_view, a_view, rsa);
+                    }
+                    LemmaMulIsAssociativeAuto();
+                }
+            IsModEquivalent(next_a, next_goal * rsa.R_INV * rsa.R, m);
+                { r_r_inv_cancel_lemma(next_a, next_goal, rsa); }
+            IsModEquivalent(next_a, next_goal, m);
+        }
+    }
+
+    lemma modexp_var_inv_post_lemma(
+        a_view: seq<uint>,
+        next_a_view: seq<uint>,
+        sig: seq<uint>,
+        rsa: rsa_params)
+
+        requires montmul_inv(next_a_view, a_view, NUM_WORDS, sig, rsa);
+        requires modexp_var_inv(to_nat(a_view), to_nat(sig), rsa.E0, rsa);
+        ensures IsModEquivalent(to_nat(next_a_view), Pow(to_nat(sig), rsa.E), rsa.M);
+    {
+        var m := rsa.M;
+        var a := to_nat(a_view);
+        var next_a := to_nat(next_a_view);
+        var s := to_nat(sig);
+
+        LemmaPowPositiveAuto();
+        // LemmaPowNonnegativeAuto();
+        var cur := Pow(s, Pow(2, rsa.E0));
+
+        assert IsModEquivalent(a, cur * rsa.R, m);
+
+        calc ==> {
+            IsModEquivalent(a, cur * rsa.R, m);
+                { LemmaModMulEquivalentAuto(); }
+            IsModEquivalent(a * (s * rsa.R_INV), (cur * rsa.R) * (s * rsa.R_INV), m);
+                { LemmaMulIsAssociativeAuto(); }
+            IsModEquivalent(a * s * rsa.R_INV, cur * rsa.R * s * rsa.R_INV, m);
+                {
+                    assert IsModEquivalent(next_a, a * s * rsa.R_INV, m) by {
+                        montmul_inv_lemma_1(next_a_view, a_view, sig, rsa);
+                    }
+                }
+            IsModEquivalent(next_a, cur * rsa.R * s * rsa.R_INV, m);
+                {
+                    LemmaMulProperties();
+                    r_r_inv_cancel_lemma(next_a, cur * s, rsa);
+                }
+            IsModEquivalent(next_a, cur * s, m);
+                {
+                    LemmaMulIsCommutativeAuto();
+                    reveal Pow();
+                }
+            IsModEquivalent(next_a, Pow(s, Pow(2, rsa.E0) + 1), m);
+            IsModEquivalent(next_a, Pow(s, rsa.E), m);
+            IsModEquivalent(to_nat(next_a_view), Pow(to_nat(sig), rsa.E), m);
+        }
+    }
+
+    lemma modexp_var_correct_lemma(
+        raw_val: nat,
+        adjusted_val: nat,
+        carry: bool,
+        rsa: rsa_params)
+
+    requires rsa_params_inv(rsa);
+    requires raw_val < rsa.SIG + rsa.M;
+    requires IsModEquivalent(raw_val, Pow(rsa.SIG, rsa.E), rsa.M);
+    requires carry ==> raw_val < rsa.M;
+    requires !carry ==> raw_val - rsa.M == adjusted_val;
+
+    ensures carry ==> raw_val == Pow(rsa.SIG, rsa.E) % rsa.M;
+    ensures !carry ==> adjusted_val == Pow(rsa.SIG, rsa.E) % rsa.M;
+    {
+        if carry {
+            LemmaSmallMod(raw_val, rsa.M);
+            assert raw_val == Pow(rsa.SIG, rsa.E) % rsa.M;
+        } else {
+            calc ==> {
+                true;
+                    { LemmaSubModNoopRight(raw_val, rsa.M as int, rsa.M); }
+                IsModEquivalent(raw_val, adjusted_val, rsa.M);
+                IsModEquivalent(adjusted_val, Pow(rsa.SIG, rsa.E), rsa.M);
+            }
+
+            LemmaSmallMod(adjusted_val, rsa.M);
+        }
+    }
+
+/* end section on mont mod exp */
 
 }
 
 module bv256_mm_lemmas refines generic_mm_lemmas {
     import opened GBV = bv256_ops
+    import opened ot_machine
+
+    type uint512_view_t = dw_view_t
+
+    predicate valid_uint512_view(
+        wdrs: wdrs_t, num: uint512_view_t,
+        li: int, ui: int)
+        requires -1 <= li < BASE_5;
+        requires -1 <= ui < BASE_5;
+    {
+        && (li == NA || wdrs[li] == num.lh)
+        && (ui == NA || wdrs[ui] == num.uh)
+    }
 
     const NUM_WORDS := 12
+
+    const B  : int := BASE_64;
+    const B2 : int := B * B;
+    const B3 : int := B * B * B;
+    const B4 : int := B * B * B * B;
+    const B5 : int := B * B * B * B * B;
+    const B6 : int := B * B * B * B * B * B;
+    const B8 : int := B4 * B4;
+
+    lemma mul256_correct_lemma(
+        p0: uint256,
+        p1: uint256,
+        p2: uint256,
+        p3: uint256,
+        p4: uint256,
+        p5: uint256,
+        p6: uint256,
+        p7: uint256,
+        p8: uint256,
+        p9: uint256,
+        p10: uint256,
+        p11: uint256,
+        p12: uint256,
+        p13: uint256,
+        p14: uint256,
+        p15: uint256,
+        r0: uint256,
+        r1: uint256,
+        r2: uint256,
+        r3: uint256,
+
+        x: uint256,
+        y: uint256,
+
+        t0: uint256,
+        t1: uint256,
+        t2: uint256,
+        u0: uint256,
+        u1: uint256,
+        u2: uint256,
+        wacc: uint256)
+
+        requires
+            && p0 == otbn_qmul(x, 0, y, 0)
+            && p1 == otbn_qmul(x, 1, y, 0)
+            && p2 == otbn_qmul(x, 0, y, 1)
+            && p3 == otbn_qmul(x, 2, y, 0)
+            && p4 == otbn_qmul(x, 1, y, 1)
+            && p5 == otbn_qmul(x, 0, y, 2)
+            && p6 == otbn_qmul(x, 3, y, 0)
+            && p7 == otbn_qmul(x, 2, y, 1)
+            && p8 == otbn_qmul(x, 1, y, 2)
+            && p9 == otbn_qmul(x, 0, y, 3)
+            && p10 == otbn_qmul(x, 3, y, 1)
+            && p11 == otbn_qmul(x, 2, y, 2)
+            && p12 == otbn_qmul(x, 1, y, 3)
+            && p13 == otbn_qmul(x, 3, y, 2)
+            && p14 == otbn_qmul(x, 2, y, 3)
+            && p15 == otbn_qmul(x, 3, y, 3)
+            && r0 == p0 + (p1 + p2) * B
+            && r1 == uh(r0) + p3 + p4 + p5 + (p6 + p7 + p8 + p9) * B
+            && r2 == uh(r1) + p10 + p11 + p12 + (p13 + p14) * B
+            && r3 == uh(r2) + p15
+            && t1 == otbn_hwb(t0, lh(r0), true)
+            && t2 == otbn_hwb(t1, lh(r1), false)
+            && u1 == otbn_hwb(u0, lh(r2), true)
+            && u2 == otbn_hwb(u1, lh(r3), false)
+            && wacc == uh(r3)
+
+        ensures
+            to_nat([t2, u2]) == x * y;
+    {
+        assert t2 == lh(r0) + lh(r1) * B2 by {
+            otbn_hwb_lemma(t0, t1, t2, lh(r0), lh(r1));
+        }
+
+        assert u2 == lh(r2) + lh(r3) * B2 by {
+            otbn_hwb_lemma(u0, u1, u2, lh(r2), lh(r3));
+        }
+
+        assert x == otbn_qsel(x, 0) + otbn_qsel(x, 1) * B + otbn_qsel(x, 2) * B2 + otbn_qsel(x, 3) * B3 by {
+            uint256_quarter_split_lemma(x);
+        }
+
+        assert y == otbn_qsel(y, 0) + otbn_qsel(y, 1) * B + otbn_qsel(y, 2) * B2 + otbn_qsel(y, 3) * B3 by {
+            uint256_quarter_split_lemma(y);
+        }
+
+        calc {
+            t2 + u2 * B4 + wacc * B8;
+                { half_split_lemma(r3); }
+            t2 + (lh(r2) + r3 * B2) * B4;
+                { half_split_lemma(r2); }
+            t2 + (r2 - uh(r2) * B2 + r3 * B2) * B4;
+            t2 + r2 * B4 - uh(r2) * B2 * B4 + r3 * B2 * B4;
+            lh(r0) + lh(r1) * B2 + r2 * B4 - uh(r2) * B2 * B4 + r3 * B2 * B4;
+                { LemmaMulIsAssociativeAuto(); }
+            lh(r0) + lh(r1) * B2 + r2 * B4 + (r3 - uh(r2)) * B6;
+            lh(r0) + lh(r1) * B2 + r2 * B4 + p15 * B6;
+                { half_split_lemma(r1); }
+            lh(r0) + r1 * B2 + (p10 + p11 + p12) * B4 + (p13 + p14) * B5 + p15 * B6;
+                { half_split_lemma(r0); }
+            p0 + (p1 + p2) * B + (p3 + p4 + p5) * B2 + (p6 + p7 + p8 + p9) * B3 + (p10 + p11 + p12) * B4 + (p13 + p14) * B5 + p15 * B6;
+                {
+                    reveal otbn_qmul();
+                    LemmaMulProperties();
+                    assume false;
+                }
+            x * y;
+        }
+
+        assert wacc == 0 by {
+            assume false;
+            // single_digit_lemma_0(x, y, B4-1);
+            // assert x * y <= B8;
+        }
+
+        assert to_nat([t2, u2]) == x * y by {
+            GBV.BVSEQ.LemmaSeqLen2([t2, u2]);
+        }
+    }
 }
