impl/dafny/bv256_dw_add.i.dfy
@@ -1,8 +1,0 @@
-include "../dafny/generic_dw_add.i.dfy"
-include "../../arch/otbn/abstraction.i.dfy"
-include "../../lib/bv256_ops.dfy"
-
-module bv256_dw_add refines generic_dw_add {
-    import opened GBV = bv256_ops
-    // import opened BVSEQ = GBV.BVSEQ
-}
